Updated case study. Missing full implementation of MakeWithdrawal and SystemInvariant.

impl/examples/cash_machine.thy
@@ -1,77 +1,157 @@
 section {* Cash Machine Case Study *}
 
 theory cash_machine
-  imports "../utp_impl" Set
+  imports "../utp_impl" Set 
 begin
 
-datatype validateResult = PinOk | PinNotOk | Retained
+text {*
+  The following is necessary to step through alphabeths, 
+  e.g. alphabet1field:alphabet2field
+ *}
+syntax
+  "_ulens_expr" :: "logic \<Rightarrow> svid \<Rightarrow> logic" ("_:'(_')" [100,100] 100)
 
+translations
+  "_ulens_expr e x" == "CONST uop get\<^bsub>x\<^esub> e"
+
+datatype ValidateResult = PinOk | PinNotOk | Retained
 type_synonym Name = string
 type_synonym AccountId = nat
 type_synonym Code = nat
 type_synonym CardId = nat
 type_synonym PinCode = nat
+type_synonym Date = string
 
-record Cardholder = 
+alphabet Transaction_st = 
+        dateT :: Date
+        cardIdT :: CardId
+        amountT :: nat
+
+alphabet Cardholder = 
   name :: Name
 
-record Card = 
+alphabet Card_st = 
   code :: Code
   cardId :: CardId
   accountId :: AccountId
 
-term "make"
-
-record Account = 
+alphabet Account_st = 
   cards :: "(CardId, Cardholder) pfun"
   balance :: nat
+  transactions :: "Transaction_st list"
   
 alphabet cm_st =
-  accounts     :: "(AccountId, Account) pfun"
+  accounts     :: "(AccountId, Account_st) pfun"
   illegalCards :: "CardId set"
-  curCard      :: "Card option"
+  curCard      :: "Card_st option"
   cardOk       :: "bool"
-  retainedCards :: "Card set"
-  (*TODO: How do I return this from getBalance()?*)
+  retainedCards :: "Card_st set"
+  local :: Card_st
+  validateReturn :: ValidateResult
   balanceReturn :: nat
 
-definition IsLegalCard :: "Card \<Rightarrow> CardId set \<Rightarrow> (AccountId, Account) pfun \<Rightarrow> bool" where
-"IsLegalCard mcard pillegalCards paccounts = 
-  (((cardId mcard) \<notin> pillegalCards) \<and> 
-  ((accountId mcard) \<in> (pdom paccounts)) \<and> 
-  ((cardId mcard) \<in> (pdom (cards (paccounts(accountId mcard)\<^sub>p)))))"
+declare [[show_types]]
 
-(* TODO: Should this be regular HOL or UTP? *)
-definition Encode :: "PinCode \<Rightarrow> nat" where
-"Encode pin = pin" (* TBD *)
+subsection {* Utilities *}
+definition mk_transaction :: "char list * nat * nat \<Rightarrow> Transaction_st" where
+[prog_defs]: "mk_transaction = (\<lambda> (xs, i, j). Transaction_st.make xs i j)"
 
-definition InsertCard :: "Card \<Rightarrow> cm_st prog" where
-[prog_defs]: "InsertCard(c) = ({&curCard =\<^sub>u \<guillemotleft>None\<guillemotright>}\<^sub>p ; curCard := \<guillemotleft>Some(c)\<guillemotright>)"
+subsection {* Functions and Invariants *}
 
-lemma "curCard := \<guillemotleft>Some undefined\<guillemotright> ; InsertCard(c) = abort" 
-  by (peq)
+(* TODO: cm_st_inv is to be replaced by SystemInvariant *)
+definition [prog_defs]: "cm_st_inv = (
+  &curCard =\<^sub>u \<guillemotleft>None\<guillemotright> \<Rightarrow> \<not> &cardOk 
+)"
 
-lemma "curCard := \<guillemotleft>None\<guillemotright> ; InsertCard(c); InsertCard(d) = abort"
-  by (peq)
+definition SystemInvariant :: "(AccountId, Account_st) pfun * Card_st option * bool \<Rightarrow> _" where
+[prog_defs]: "SystemInvariant = (\<lambda>(accs, cardP, cardOkP) . 
+  ((cardP = None \<longrightarrow> \<not> cardOkP) \<and> 
+  (\<forall> id1  \<in> (pdom accs) . (\<forall> id2 \<in> (pdom accs) . (id1 \<noteq> id2) \<longrightarrow> 
+  (pdom (cards\<^sub>v(accs(id1)\<^sub>p)) \<inter> pdom (cards\<^sub>v(accs(id1)\<^sub>p)) = {})))))"
 
-term "the (\<lbrakk>&curCard\<rbrakk>\<^sub>e cm_st)"
-term "\<guillemotleft>code o the\<guillemotright>(&curCard)\<^sub>a"
+definition DateTotal :: "Date * Transaction_st list \<Rightarrow> nat" where
+[prog_defs]: "DateTotal  = (\<lambda>(d, ts) . foldl (\<lambda> (acc::nat) (x::Transaction_st) . 
+  if (dateT\<^sub>v x = (d::Date)) then acc + amountT\<^sub>v x else acc) 
+  (0::nat) (ts::Transaction_st list))"
 
-term "trop IsLegalCard"
-term "(&curCard)"
-term "\<guillemotleft>the\<guillemotright>"
-term "\<guillemotleft>the\<guillemotright> (&curCard)\<^sub>a"
+definition TransactionsInvariant :: "Transaction_st list \<Rightarrow> bool" where
+[prog_defs]: "TransactionsInvariant ts = (\<forall> d \<in> List.coset(map (\<lambda>x . dateT\<^sub>v x) ts) . DateTotal(d,ts) < 200)"
 
+definition IsLegalCard :: "Card_st * CardId set * (AccountId, Account_st) pfun \<Rightarrow> bool" where
+[prog_defs]: "IsLegalCard = (\<lambda>(mcard, pillegalCards, paccounts) .
+  (((cardId\<^sub>v mcard) \<notin> pillegalCards) \<and> 
+  ((accountId\<^sub>v mcard) \<in> (pdom paccounts)) \<and> 
+  ((cardId\<^sub>v mcard) \<in> (pdom (cards\<^sub>v (paccounts(accountId\<^sub>v mcard)\<^sub>p))))))"
 
-(* TODO: Return a value *)
-definition Validate :: "PinCode \<Rightarrow> cm_st prog" where
-"Validate pin = ( 
-  let codeOK::bool = (\<guillemotleft>code o the\<guillemotright>(&curCard)\<^sub>a) = \<guillemotleft>(Encode(pin))\<guillemotright> in
-      let cardLegal = (trop IsLegalCard) (\<guillemotleft>the\<guillemotright> (&curCard)\<^sub>a) (&illegalCards) (&accounts) in 
-        if (\<not>cardLegal) then (retainedCards := (&retainedCards \<union>\<^sub>u {(&curCard)}\<^sub>u)) else (retainedCards := &retainedCards))"
+definition Encode :: "PinCode \<Rightarrow> PinCode" where
+[prog_defs]: "Encode = id"
+
+definition Sum :: "real list \<Rightarrow> real" where
+[prog_defs]: "Sum = sum_list"
+
+subsection {* Operations *}
+
+definition InsertCard :: "Card_st \<Rightarrow> cm_st prog" where
+[prog_defs]: "InsertCard c = ({&curCard =\<^sub>u \<guillemotleft>None\<guillemotright>}\<^sub>p ; curCard := (uop Some)\<guillemotleft>c\<guillemotright>)"
+
+definition Validate :: "(ValidateResult \<Longrightarrow> 'a cm_st_scheme) \<Rightarrow> PinCode \<Rightarrow> 'a cm_st_scheme prog" where
+[prog_defs]: "Validate ret p = ({&curCard \<noteq>\<^sub>u \<guillemotleft>None\<guillemotright> \<and> \<not> &cardOk}\<^sub>p;(
+  let codeOk =  (uop the)&curCard:(code) =\<^sub>u \<guillemotleft>Encode(p)\<guillemotright> in 
+    let cardLegal = \<guillemotleft>IsLegalCard\<guillemotright>((\<guillemotleft>the\<guillemotright> (&curCard)\<^sub>a, &illegalCards, &accounts)\<^sub>u)\<^sub>a in
+      if (\<not> cardLegal) 
+      \<rightarrow> (retainedCards := (&retainedCards \<union>\<^sub>u {(uop the) &curCard}\<^sub>u);
+        cardOk := false;curCard := \<guillemotleft>None\<guillemotright>; ret := \<guillemotleft>Retained\<guillemotright>) 
+      else cardOk := codeOk;if &cardOk \<rightarrow> ret := \<guillemotleft>PinOk\<guillemotright>  else ret := \<guillemotleft>PinNotOk\<guillemotright> fi fi))"
 
 definition ReturnCard :: "cm_st prog" where
 [prog_defs]: "ReturnCard = ({&curCard \<noteq>\<^sub>u \<guillemotleft>None\<guillemotright>}\<^sub>p; cardOk := false ; curCard := \<guillemotleft>None\<guillemotright>)"
+
+definition GetBalance :: "(nat \<Longrightarrow> cm_st) \<Rightarrow> cm_st prog" where
+[prog_defs]: "GetBalance ret = (
+  {&curCard \<noteq>\<^sub>u \<guillemotleft>None\<guillemotright> \<and> &cardOk \<and> 
+  \<guillemotleft>IsLegalCard\<guillemotright>((\<guillemotleft>the\<guillemotright> (&curCard)\<^sub>a, &illegalCards, &accounts)\<^sub>u)\<^sub>a}\<^sub>p; 
+  ret := (&accounts((\<guillemotleft>the\<guillemotright>(&curCard)\<^sub>a):(accountId))\<^sub>a):(balance))"
+
+(* TODO: MakeWithdrawal needs an implementation on 
+  (&accounts(accountIdL)\<^sub>a):(balance) := \<guillemotleft>1\<guillemotright>
+*)
+
+definition MakeWithdrawal :: "nat \<Rightarrow> Date \<Rightarrow> _ \<Rightarrow> _" where
+[prog_defs]: "MakeWithdrawal amountP dateP ret = 
+   {&curCard \<noteq>\<^sub>u \<guillemotleft>None\<guillemotright> \<and> &cardOk \<and> \<guillemotleft>IsLegalCard\<guillemotright>((\<guillemotleft>the\<guillemotright> (&curCard)\<^sub>a, &illegalCards, &accounts)\<^sub>u)\<^sub>a}\<^sub>p;
+  (let cardIdL = (uop the)&curCard:(cardId) 
+  in 
+    let accountIdL = (uop the)&curCard:(accountId)
+    in 
+      let transactionL = \<guillemotleft>mk_transaction\<guillemotright>(\<guillemotleft>dateP\<guillemotright>, cardIdL, \<guillemotleft>amountP\<guillemotright>)\<^sub>a 
+      in
+        let allTransL = &accounts(accountIdL)\<^sub>a:(transactions) ^\<^sub>u \<langle>transactionL\<rangle> 
+        in (
+          if (((&accounts(accountIdL)\<^sub>a):(balance) - \<guillemotleft>amountP\<guillemotright> \<ge>\<^sub>u \<guillemotleft>0\<guillemotright>) \<and> (\<guillemotleft>DateTotal\<guillemotright>(\<guillemotleft>dateP\<guillemotright>, allTransL)\<^sub>a \<le>\<^sub>u \<guillemotleft>200\<guillemotright>)) \<rightarrow>
+             (ret := true;undefined) 
+          else ret := false;undefined
+          fi ))"
+
+definition RequestStatement :: "_" where 
+[prog_defs]: "RequestStatement ret = 
+  {&curCard \<noteq>\<^sub>u \<guillemotleft>None\<guillemotright> \<and> &cardOk \<and> \<guillemotleft>IsLegalCard\<guillemotright>((\<guillemotleft>the\<guillemotright> (&curCard)\<^sub>a, &illegalCards, &accounts)\<^sub>u)\<^sub>a}\<^sub>p;
+  (let acc = &accounts((uop the) &curCard:(accountId))\<^sub>a in 
+    let c = acc:(cards) in 
+      ret := (c(uop the &curCard:(accountId))\<^sub>a:(name), acc:(transactions), acc:(balance))\<^sub>u)"
+
+definition ReportIllegalCard :: "(CardId, cm_st) uexpr \<Rightarrow> cm_st prog" where
+[prog_defs]: "ReportIllegalCard cId = (illegalCards := (&illegalCards \<union>\<^sub>u {cId}\<^sub>u))"
+
+definition AddAccount :: "(AccountId, cm_st) uexpr \<Rightarrow> (Account_st, cm_st) uexpr \<Rightarrow> cm_st prog" where
+[prog_defs]: "AddAccount accId acc = ({accId \<notin>\<^sub>u uop pdom &accounts}\<^sub>p;accounts := &accounts(accId \<mapsto> acc)\<^sub>u)"
+
+subsection {* Proofs *}
+
+lemma "\<Sigma>:[cm_st_inv \<and> &curCard =\<^sub>u \<guillemotleft>None\<guillemotright>, cm_st_inv] \<sqsubseteq> InsertCard(c)"
+  by (prefine)
+
+lemma "curCard := \<guillemotleft>Some undefined\<guillemotright> ; InsertCard(c) = abort" 
+  by (peq)
 
 lemma "curCard := \<guillemotleft>None\<guillemotright> ; ReturnCard = abort"
   by (peq)
@@ -79,37 +159,17 @@ lemma "curCard := \<guillemotleft>None\<guillemotright> ; ReturnCard = abort"
 lemma "curCard := \<guillemotleft>Some(c)\<guillemotright> ; ReturnCard; ReturnCard = abort"
   by (peq)
 
-(*lemma "curCard := \<guillemotleft>Some(c)\<guillemotright> ; ReturnCard \<noteq> abort"
-  by (peq)*)
-
-term "accountId o the"
-term "(\<guillemotleft>accountId o the\<guillemotright> (&curCard)\<^sub>a) "
-term "\<guillemotleft>1\<guillemotright>"
-
-term "(&accounts ((\<guillemotleft>accountId o the\<guillemotright> (&curCard)\<^sub>a) )\<^sub>a )"
-term "(\<guillemotleft>balance\<guillemotright> (&accounts ((\<guillemotleft>accountId o the\<guillemotright> (&curCard)\<^sub>a))\<^sub>a)\<^sub>a)"
-
-definition GetBalance :: "cm_st prog" where
-[prog_defs]: "GetBalance = {&curCard \<noteq>\<^sub>u \<guillemotleft>None\<guillemotright>}\<^sub>p ; balanceReturn := \<guillemotleft>balance\<guillemotright> (&accounts((\<guillemotleft>accountId o the\<guillemotright>(&curCard)\<^sub>a))\<^sub>a)\<^sub>a"
-
-(*
-definition GetBalanceFun :: "cm_st \<Rightarrow> nat" where
-"GetBalanceFun = \<lbrakk>\<guillemotleft>balance\<guillemotright> (&accounts((\<guillemotleft>accountId o the\<guillemotright>(&curCard)\<^sub>a))\<^sub>a)\<^sub>a\<rbrakk>\<^sub>e"
-
-definition GetBalanceApp :: "cm_st prog" where [prog_defs]:
-"GetBalanceApp = {&curCard \<noteq>\<^sub>u \<guillemotleft>None\<guillemotright>}\<^sub>p ; balanceReturn := (Abs_uexpr GetBalanceFun)"*)
-
-definition ReportIllegalCard :: "CardId \<Rightarrow> cm_st prog" where
-[prog_defs]: "ReportIllegalCard cId = (illegalCards := (&illegalCards \<union>\<^sub>u {\<guillemotleft>cId\<guillemotright>}\<^sub>u))"
-
-definition AddAccount :: "AccountId \<Rightarrow> Account \<Rightarrow> cm_st prog" where
-[prog_defs]: "AddAccount accId acc = 
-  ({\<guillemotleft>accId\<guillemotright> \<notin>\<^sub>u dom\<^sub>u(&accounts)}\<^sub>p; 
-  accounts := &accounts(\<guillemotleft>accId\<guillemotright> \<mapsto> \<guillemotleft>acc\<guillemotright>)\<^sub>u)"
+subsection {* Notes *}
+(* Example of forall in UTP *)
+term
+ "\<^bold>\<forall> id1\<in>dom\<^sub>u(accountsP::((nat, Account_st) pfun, 'a cm_st_scheme) uexpr) \<bullet>
+  \<^bold>\<forall> id2\<in>dom\<^sub>u(accountsP::((nat, Account_st) pfun, 'a cm_st_scheme) uexpr) \<bullet> \<guillemotleft>id1\<guillemotright> \<noteq>\<^sub>u \<guillemotleft>id2\<guillemotright>"
 
 
+(* Example of using mk_transaction *)
+term "\<guillemotleft>mk_transaction\<guillemotright>(\<langle>\<rangle>, 0, &x)\<^sub>a"
 
-
-
+(* Example of updating a mapping *)
+term "accounts := &accounts(\<guillemotleft>aid\<guillemotright> \<mapsto> &accounts(\<guillemotleft>aid\<guillemotright>)\<^sub>a)\<^sub>u"
 
 end
