impl/examples/cash_machine_old.thy
@@ -1,0 +1,356 @@
+section {* Cash Machine Case Study *}
+text {*
+  Names ending with 2 represents a full utp approach, where alphabets are used.
+  The other approach is using e.g. ordinary records.
+*}
+theory cash_machine
+  imports "../utp_impl" Set 
+begin
+
+text {*
+  The following is necessary to step through alphabeths, 
+  e.g. alphabet1field:alphabet2field
+ *}
+syntax
+  "_ulens_expr" :: "logic \<Rightarrow> svid \<Rightarrow> logic" ("_:'(_')" [100,100] 100)
+
+translations
+  "_ulens_expr e x" == "CONST uop get\<^bsub>x\<^esub> e"
+
+datatype ValidateResult = PinOk | PinNotOk | Retained
+type_synonym Name = string
+type_synonym AccountId = nat
+type_synonym Code = nat
+type_synonym CardId = nat
+type_synonym PinCode = nat
+type_synonym Date = string
+
+alphabet Transaction_st = 
+        dateT :: Date
+        cardIdT :: CardId
+        amountT :: nat
+
+alphabet Cardholder = 
+  name :: Name
+
+record Card = 
+  code :: Code
+  cardId :: CardId
+  accountId :: AccountId
+
+alphabet Card_st = 
+  code2 :: Code
+  cardId2 :: CardId
+  accountId2 :: AccountId
+
+
+term "make"
+
+record Account = 
+  cards :: "(CardId, Cardholder) pfun"
+  balance :: nat
+
+alphabet Account_st = 
+  cards2 :: "(CardId, Cardholder) pfun"
+  balance2 :: nat
+  transactions2 :: "Transaction_st list"
+  
+alphabet cm_st =
+  accounts     :: "(AccountId, Account) pfun"
+  accounts2     :: "(AccountId, Account_st) pfun"
+  illegalCards :: "CardId set"
+  curCard      :: "Card option"
+  curCard2      :: "Card_st option"
+  cardOk       :: "bool"
+  retainedCards :: "Card set"
+  retainedCards2 :: "Card_st set"
+  local         :: nat
+  local2 :: Card_st
+  validateReturn :: ValidateResult
+  balanceReturn :: nat
+
+definition [prog_defs]: "cm_st_inv = (
+  &curCard =\<^sub>u \<guillemotleft>None\<guillemotright> \<Rightarrow> \<not> &cardOk 
+)"
+
+subsection {* todo: *}
+text {* 
+  mk_System_inv: forall x in ((nat set, 'a cm_st_scheme) uexpr) . pred x
+  Withdrawal: Combining multiple alphabets in sequential composition? 
+  Withdrawal: Creating a new instance of an alphabet?
+*}
+
+declare [[show_types]]
+
+term
+ "\<^bold>\<forall> id1\<in>dom\<^sub>u(accountsP::((nat, Account_st) pfun, 'a cm_st_scheme) uexpr) \<bullet>
+  \<^bold>\<forall> id2\<in>dom\<^sub>u(accountsP::((nat, Account_st) pfun, 'a cm_st_scheme) uexpr) \<bullet> \<guillemotleft>id1\<guillemotright> \<noteq>\<^sub>u \<guillemotleft>id2\<guillemotright>"
+
+(*
+definition mk_System_inv :: "((nat, Account_st) pfun, 'a cm_st_scheme) uexpr \<Rightarrow> (Card_st option, 'a cm_st_scheme) uexpr \<Rightarrow> (bool, 'a cm_st_scheme) uexpr \<Rightarrow> (bool, 'a cm_st_scheme) uexpr" where
+"mk_System_inv accountsP curCardP cardOkP = (
+  (curCardP =\<^sub>u \<guillemotleft>None\<guillemotright> \<Rightarrow> \<not> cardOkP) \<and>
+  (\<forall> (id1 \<in> (\<lbrakk>dom\<^sub>u(accountsP)\<rbrakk>\<^sub>e)) \<bullet> 
+)"
+*)
+
+(* 
+inv mk_System(accs,-,curCard,cardOk,-) == 
+      (curCard = nil => not cardOk) and 
+      (forall id1, id2 in set dom accs &
+        id1 <> id2 =>
+        dom accs(id1).cards inter dom accs(id2).cards = {})
+*)
+
+definition IsLegalCard2 :: "(Card_st, 'a cm_st_scheme) uexpr \<Rightarrow> (CardId set, 'a cm_st_scheme) uexpr \<Rightarrow> (((nat, Account_st) pfun, 'a cm_st_scheme) uexpr) \<Rightarrow> (bool, 'a cm_st_scheme) uexpr" where
+[prog_defs]: "IsLegalCard2 c cSet acc = 
+  (((c:(cardId2)) \<notin>\<^sub>u cSet) \<and> 
+  ((c:(accountId2)) \<in>\<^sub>u dom\<^sub>u(acc)) \<and>
+    ((c:(cardId2)) \<in>\<^sub>u dom\<^sub>u((acc(c:(accountId2))\<^sub>a):(cards2))))"
+
+definition IsLegalCard :: "Card \<Rightarrow> CardId set \<Rightarrow> (AccountId, Account) pfun \<Rightarrow> bool" where
+"IsLegalCard mcard pillegalCards paccounts = 
+  (((cardId mcard) \<notin> pillegalCards) \<and> 
+  ((accountId mcard) \<in> (pdom paccounts)) \<and> 
+  ((cardId mcard) \<in> (pdom (cards (paccounts(accountId mcard)\<^sub>p)))))"
+
+definition Encode2 :: "(PinCode, cm_st) uexpr \<Rightarrow> (PinCode, cm_st) uexpr" where
+[prog_defs]: "Encode2 p = p"
+
+definition Encode :: "PinCode \<Rightarrow> nat" where
+"Encode pin = pin"
+term "\<guillemotleft>Card\<guillemotright>"
+
+definition InsertCard2 :: "(Card_st, cm_st) uexpr \<Rightarrow> cm_st prog" where
+[prog_defs]: "InsertCard2 c = ({&curCard2 =\<^sub>u \<guillemotleft>None\<guillemotright>}\<^sub>p ; curCard2 := (uop Some)c)"
+
+definition InsertCard :: "Card \<Rightarrow> cm_st prog" where
+[prog_defs]: "InsertCard(c) = ({&curCard =\<^sub>u \<guillemotleft>None\<guillemotright>}\<^sub>p ; curCard := \<guillemotleft>Some(c)\<guillemotright>)"
+
+term "x:[P, \<guillemotleft>iv\<guillemotright>:(local) >\<^sub>u &local]"
+
+lemma "\<Sigma>:[cm_st_inv \<and> &curCard =\<^sub>u \<guillemotleft>None\<guillemotright>, cm_st_inv] \<sqsubseteq> InsertCard(c)"
+  by (prefine)
+
+lemma "curCard := \<guillemotleft>Some undefined\<guillemotright> ; InsertCard(c) = abort" 
+  by (peq)
+
+
+definition Validate2 :: "(PinCode, cm_st) uexpr \<Rightarrow> cm_st prog" where
+[prog_defs]: "Validate2 pin_uexpr = (
+  {&curCard2 \<noteq>\<^sub>u \<guillemotleft>None\<guillemotright> \<and> &cardOk =\<^sub>u false}\<^sub>p;
+  (let codeOk::cm_st upred = (uop the)&curCard2:(code2) =\<^sub>u Encode2(pin_uexpr) in 
+    let cardLegal::(bool, cm_st) uexpr = IsLegalCard2 (\<guillemotleft>the\<guillemotright> (&curCard2)\<^sub>a) &illegalCards &accounts2 in 
+      if (cardLegal = false) 
+      then retainedCards2 := (&retainedCards2 \<union>\<^sub>u {(uop the) &curCard2}\<^sub>u);cardOk := false;curCard2 := \<guillemotleft>None\<guillemotright>;validateReturn := \<guillemotleft>Retained\<guillemotright>
+      else cardOk := codeOk;
+        (if (&cardOk = true)
+        then (validateReturn := \<guillemotleft>PinOk\<guillemotright>)
+        else (validateReturn := \<guillemotleft>PinNotOk\<guillemotright>))))"
+
+definition Validate :: "PinCode \<Rightarrow> cm_st prog" where
+[prog_defs]: "Validate pin =  (
+  let codeOk = (\<guillemotleft>code o the\<guillemotright>(&curCard)\<^sub>a) =\<^sub>u \<guillemotleft>Encode(pin)\<guillemotright> in
+    let cardLegal = (trop IsLegalCard) (\<guillemotleft>the\<guillemotright> (&curCard)\<^sub>a) (&illegalCards) (&accounts) in 
+      ( if(cardLegal = false) 
+        then (retainedCards := (&retainedCards \<union>\<^sub>u {\<guillemotleft>the\<guillemotright> (&curCard)\<^sub>a}\<^sub>u);
+          cardOk := false; 
+          curCard := \<guillemotleft>None\<guillemotright>; 
+          validateReturn := \<guillemotleft>Retained\<guillemotright>)
+        else (cardOk := codeOk;(
+          if (&cardOk = true) 
+          then (validateReturn := \<guillemotleft>PinOk\<guillemotright>) 
+          else (validateReturn := \<guillemotleft>PinNotOk\<guillemotright>)))))"
+
+definition ReturnCard2 :: "cm_st prog" where
+[prog_defs]: "ReturnCard2 = ({&curCard2 \<noteq>\<^sub>u \<guillemotleft>None\<guillemotright>}\<^sub>p; cardOk := false ; curCard2 := \<guillemotleft>None\<guillemotright>)"
+
+definition ReturnCard :: "cm_st prog" where
+[prog_defs]: "ReturnCard = ({&curCard \<noteq>\<^sub>u \<guillemotleft>None\<guillemotright>}\<^sub>p; cardOk := false ; curCard := \<guillemotleft>None\<guillemotright>)"
+
+lemma "curCard := \<guillemotleft>None\<guillemotright> ; ReturnCard = abort"
+  by (peq)
+
+lemma "curCard := \<guillemotleft>Some(c)\<guillemotright> ; ReturnCard; ReturnCard = abort"
+  by (peq)
+
+definition GetBalance2 :: "cm_st prog" where
+[prog_defs]: "GetBalance2 = (
+  {&curCard2 \<noteq>\<^sub>u \<guillemotleft>None\<guillemotright> \<and> &cardOk =\<^sub>u true \<and> 
+  IsLegalCard2 (uop the &curCard2) &illegalCards &accounts2 =\<^sub>u true}\<^sub>p; 
+  balanceReturn := (&accounts2((\<guillemotleft>the\<guillemotright>(&curCard2)\<^sub>a):(accountId2))\<^sub>a):(balance2))"
+
+definition GetBalance :: "cm_st prog" where
+[prog_defs]: "GetBalance = {&curCard \<noteq>\<^sub>u \<guillemotleft>None\<guillemotright>}\<^sub>p ; balanceReturn := \<guillemotleft>balance\<guillemotright> (&accounts((\<guillemotleft>accountId o the\<guillemotright>(&curCard)\<^sub>a))\<^sub>a)\<^sub>a"
+
+(* Example of passing a value to return in
+definition GetBalance :: "(nat \<Longrightarrow> cm_st) \<Rightarrow> cm_st prog" where
+[prog_defs]: "GetBalance balanceReturn = {&curCard \<noteq>\<^sub>u \<guillemotleft>None\<guillemotright>}\<^sub>p ; balanceReturn := \<guillemotleft>balance\<guillemotright> (&accounts((\<guillemotleft>accountId o the\<guillemotright>(&curCard)\<^sub>a))\<^sub>a)\<^sub>a"
+
+definition Average :: "cm_st prog" where
+[prog_defs]: "Average = GetBalance local"
+*)
+(*
+ MakeWithdrawal : nat * Date ==> bool
+  MakeWithdrawal(amount,date) ==
+    let mk_Card(-,cardId,accountId) = curCard,
+        transaction = mk_Transaction(date,cardId,amount)        
+    in
+      if accounts(accountId).balance - amount >= 0 and 
+        DateTotal(date,accounts(accountId).transactions^[transaction])
+        <= dailyLimit
+      then
+        (accounts(accountId).balance := 
+           accounts(accountId).balance - amount;
+         accounts(accountId).transactions := 
+           accounts(accountId).transactions ^ [transaction];
+         return true)
+     else 
+       return false
+  pre curCard <> nil and cardOk and IsLegalCard(curCard,illegalCards,accounts);
+*)
+term "trop"
+term "filter"
+term "bop (filter)"
+term "[x \<leftarrow> [1,2,3].x>1]"
+
+text {* 
+  This cannot be defined using uexpr, 
+  because it is not possible to iterate over a uexpe containing a list 
+*}
+
+
+primrec Sum :: "(real, 'a Transaction_st_scheme) uexpr list \<Rightarrow> (real, 'a Transaction_st_scheme) uexpr" where
+"Sum (x#xs) = x + Sum(xs)" |
+"Sum [] = 0"
+
+definition DateTotal :: "Date \<Rightarrow> ((Transaction_st, 'a Transaction_st_scheme) uexpr) list \<Rightarrow> (real, 'a Transaction_st_scheme) uexpr" where
+"DateTotal dateP transactionsP = (
+  let amounts::(real, 'a Transaction_st_scheme) uexpr list = 
+    (foldl (\<lambda>xs x . if((x):(dateT) = \<guillemotleft>dateP\<guillemotright>) then ((x):(amountT))#xs else xs) 
+      [] transactionsP)
+  in Sum amounts)" 
+
+definition DateTotal2 :: "(Date, 'a Transaction_st_scheme) uexpr \<Rightarrow> ((Transaction_st, 'a Transaction_st_scheme) uexpr) list \<Rightarrow> _" where
+"DateTotal2 dateP transactionsP = (
+  (let filteredTransactions = [x <- transactionsP . (x):(dateT) = dateP] in 
+    let mappedTransactions = map (\<lambda>x . (x):(amountT)) filteredTransactions in
+      Sum mappedTransactions))"
+
+(* How do I filter  (Transaction_st list, 'a Transaction_st_scheme) uexpr? *)
+(* How do I map (Transaction_st list, 'a Transaction_st_scheme) uexpr? *)
+definition DateTotal3 :: "Date \<Rightarrow> (Transaction_st list, 'a ) uexpr \<Rightarrow> (nat, 'a ) uexpr" where
+"DateTotal3 dateP transactionsP = (
+  let filteredTransactions = uop (filter (\<lambda>x . dateT\<^sub>v x = dateP)) transactionsP in
+   (uop (\<lambda>tlist . sum_list (map amountT\<^sub>v tlist))) transactionsP)"
+
+term "(uop (\<lambda>tlist . sum_list (map amountT\<^sub>v tlist)))"
+
+term "uop (\<lambda>x::'a Transaction_st_scheme list . sum_list (map amountT\<^sub>v x))"
+term "(uop (\<lambda>x::'a Transaction_st_scheme list . sum_list (map amountT\<^sub>v x)))
+ (x::(Transaction_st list, 'a Transaction_st_scheme) uexpr)"
+
+typ "unit (Transaction_st list, 'a Transaction_st_scheme) uexpr"
+term "unit x::'a Transaction_st_scheme list"
+term "dateT"
+term "x:(dateT)"
+typ "unit ('a Transaction_st_scheme list)"
+
+find_theorems name:collect
+definition TotalAmount :: "'a Transaction_st_scheme list \<Rightarrow> nat" where
+"TotalAmount tlist = sum_list (map amountT\<^sub>v tlist)"
+
+definition TotalAmount2 :: "_" where
+"TotalAmount2 = (uop (\<lambda>tlist . sum_list (map amountT\<^sub>v tlist)))"
+term "amountT\<^sub>v"
+term "filter (\<lambda>x::'a Transaction_st_scheme . dateT\<^sub>v x = ''a'')"
+term "uop (filter (\<lambda>x::'a Transaction_st_scheme . dateT\<^sub>v x = ''a''))"
+
+typ "unit Transaction_st_scheme"
+
+term "uop TotalAmount"
+term "(uop TotalAmount) (&accounts2(1)\<^sub>a:(transactions2))"
+term "TotalAmount2 (&accounts2(1)\<^sub>a:(transactions2))"
+term "(uop length) (x::(Transaction_st list, 'a Transaction_st_scheme) uexpr) = \<guillemotleft>0\<guillemotright>"
+
+
+
+
+definition TransactionsInvariant :: "((Transaction_st, 'a Transaction_st_scheme) uexpr) list \<Rightarrow> bool" where
+"TransactionsInvariant transactionsP = (
+  let transactionDates = List.coset(map (\<lambda>x . (x):(dateT)) transactionsP) in
+    \<forall> dateP \<in> transactionDates . ((DateTotal2 dateP transactionsP) \<le>\<^sub>u \<guillemotleft>200\<guillemotright> = true))"
+
+
+(* Example of returning a nat from a state space *)
+(*definition GetBalanceFun :: "cm_st \<Rightarrow> nat" where
+"GetBalanceFun = \<lbrakk>\<guillemotleft>balance\<guillemotright> (&accounts((\<guillemotleft>accountId o the\<guillemotright>(&curCard)\<^sub>a))\<^sub>a)\<^sub>a\<rbrakk>\<^sub>e"
+
+definition GetBalanceApp :: "cm_st prog" where [prog_defs]:
+"GetBalanceApp = {&curCard \<noteq>\<^sub>u \<guillemotleft>None\<guillemotright>}\<^sub>p ; balanceReturn := (Abs_uexpr GetBalanceFun)"*)
+
+definition ReportIllegalCard2 :: "(CardId, cm_st) uexpr \<Rightarrow> cm_st prog" where
+[prog_defs]: "ReportIllegalCard2 cId = (illegalCards := (&illegalCards \<union>\<^sub>u {cId}\<^sub>u))"
+
+definition ReportIllegalCard :: "CardId \<Rightarrow> cm_st prog" where
+[prog_defs]: "ReportIllegalCard cId = (illegalCards := (&illegalCards \<union>\<^sub>u {\<guillemotleft>cId\<guillemotright>}\<^sub>u))"
+
+definition AddAccount2 :: "(AccountId, cm_st) uexpr \<Rightarrow> (Account, cm_st) uexpr \<Rightarrow> cm_st prog" where
+[prog_defs]: "AddAccount2 accId acc = (
+  {accId \<notin>\<^sub>u dom\<^sub>u(&accounts)}\<^sub>p; 
+  accounts := &accounts(accId \<mapsto> acc)\<^sub>u)"
+
+definition AddAccount :: "AccountId \<Rightarrow> Account \<Rightarrow> cm_st prog" where
+[prog_defs]: "AddAccount accId acc = 
+  ({\<guillemotleft>accId\<guillemotright> \<notin>\<^sub>u dom\<^sub>u(&accounts)}\<^sub>p; 
+  accounts := &accounts(\<guillemotleft>accId\<guillemotright> \<mapsto> \<guillemotleft>acc\<guillemotright>)\<^sub>u)"
+term "((uop the)&curCard2):(cardId2)"
+
+term "fst"
+term "snd"
+term "snd o snd"
+
+term "&accounts2((cardL):(accountId2))\<^sub>a"
+term "((x::((Cardholder, 'a cm_st_scheme) uexpr))):(name)"
+(*
+definition RequestStatement :: " _" where
+"RequestStatement = (
+  let cardIdP_accountIdP = ((uop the)&curCard2:(cardId2),(uop the)&curCard2:(accountId2)) in
+    let accountL = &accounts2((snd cardIdP_accountIdP):(accountId2))\<^sub>a in
+      let cardsP_balanceP_transactionsP = (&accountL):(cards)
+      in ( (accountL:(cards2))(cardL:(cardId2))\<^sub>a:(name),1 ))"
+*)
+(*definition RequestStatement :: "AccountId \<Rightarrow> _" where
+"RequestStatement accIdP= (
+  let cardL = (uop the) &curCard2 in
+    let accountL = &accounts2(cardL:(accountId2))\<^sub>a
+    in ( (accountL:(cards2))(cardL:(cardId2))\<^sub>a:(name),1 ))"*)
+
+
+
+term "put\<^bsub>dateT +\<^sub>L cardIdT +\<^sub>L amountT\<^esub>"
+
+definition mk_transaction :: "(char list, 'a) uexpr \<Rightarrow> (nat, 'a) uexpr \<Rightarrow>
+  (nat, 'a) uexpr \<Rightarrow> ('b Transaction_st_scheme, 'a) uexpr" where
+"mk_transaction =   trop (curry o curry (put\<^bsub>dateT +\<^sub>L cardIdT +\<^sub>L amountT\<^esub> undefined))"
+
+
+
+term "(balance2) := (&balance2)"
+
+(* TODO: How do I update balance2? *)
+definition MakeWithdrawal :: "nat \<Rightarrow> Date \<Rightarrow> _" where
+"MakeWithdrawal amountP dateP = (
+  let cardIdL = (uop the)&curCard2:(cardId2) 
+  in 
+    let accountIdL = (uop the)&curCard2:(accountId2) 
+    in 
+      let transactionL = mk_transaction \<guillemotleft>dateP\<guillemotright> cardIdL \<guillemotleft>amountP\<guillemotright> 
+      in
+        let allTransL = &accounts2(accountIdL)\<^sub>a:(transactions2) ^\<^sub>u \<langle>transactionL\<rangle> 
+        in ( 
+          if ((((&accounts2(accountIdL)\<^sub>a):(balance2) - \<guillemotleft>amountP\<guillemotright> \<ge>\<^sub>u \<guillemotleft>0\<guillemotright>) \<and> (DateTotal3 dateP allTransL \<le>\<^sub>u \<guillemotleft>200\<guillemotright>)) = true)
+          then true
+          else false))"
+
+end
